proof: add some rules

policy_proof/coq/query.v
@@ -1,20 +1,23 @@
 Require Import List.
 Require Import String.
 Require Import Unicode.Utf8.
+Require Import Lia.
 
 Require Import types.
 Require Import relation.
 Require Import formula.
 Require Import data_model.
 Require Import ordering.
+Require Import lattice.
 Require Import finite_bags.
+Require Import util.
 
 Set Printing Coercions.
 Set Printing Implicit.
 Set Printing Projections.
 
-Inductive trans_func (l1 l2: Policy.policy): Set :=
-  | trans_func_with_label: ∀ bt, transform_func bt → trans_func l1 l2
+Inductive trans_func (ℓ1 ℓ2: Policy.policy): Set :=
+  | trans_func_with_label: ∀ bt, transform_func bt → trans_func ℓ1 ℓ2
 .
 
 Fixpoint schema_to_anf (s: schema): list nat :=
@@ -60,7 +63,33 @@ Fixpoint lookup_schema (n: nat) (se: schema_env): schema :=
   This environment is used in the context of database query operations.
 *)
 Definition env_slice (s: schema) := (relation s * list nat * groupby_list * list (Tuple.tuple s))%type.
-Definition env (s: schema): Set := list (env_slice s)%type.
+Definition ℰ (s: schema): Set := list (env_slice s)%type.
+
+Definition env_slice_get_relation {s} (e: env_slice s) : relation s :=
+  match e with
+    | (r, _, _, _) => r
+  end.
+
+Definition env_slice_get_selected {s} (e: env_slice s) : list nat :=
+  match e with
+    | (_, s, _, _) => s
+  end.
+
+Definition env_slice_get_groupby {s} (e: env_slice s) : groupby_list :=
+  match e with
+    | (_, _, g, _) => g
+  end.
+
+Definition env_slice_get_tuples {s} (e: env_slice s) : list (Tuple.tuple s) :=
+  match e with
+    | (_, _, _, t) => t
+  end.
+
+Definition get_env_slice s (e: ℰ s) (non_empty: List.length e > 0) : env_slice s.
+  destruct e.
+  - simpl in non_empty. lia.
+  - exact e.
+Defined.
 
 Inductive Operator: Set :=
   | operator_empty: Operator
@@ -78,25 +107,69 @@ Inductive Operator: Set :=
 Inductive config: Set :=
   | config_terminal: config
   | config_error: config
-  | config_ok: ∀ s, Policy.context → Configuration.privacy → env s → config
+  | config_ok: ∀ s, Policy.context → Configuration.privacy → ℰ s → config
 .
+
+Notation "'⟨' s Γ β ℰ '⟩'":= (config_ok s Γ β ℰ)
+  (at level 10, s at next level, Γ at next level, β at next level, ℰ at next level,
+  no associativity).
 
 (*
   `step_cell` is an inductive type that defines a relation between two configurations except that
   it works on the level of cells. This transition is defined by a notation `c1 >[ f ]> c2` where `f`
   is a function that transforms the cell.
 *)
-Reserved Notation "c1 '>[' f ']>' c2" (at level 50, left associativity).
-Inductive step_cell: ∀ l1 l2, trans_func l1 l2 → config → config→ Prop :=
-  | E_CTransSkip:
-      ∀ l1 l2 s ctx priv (e: env s) (f: trans_func l1 l2), 
-        List.length e = 0 →
-      config_ok s ctx priv e >[ f ]> config_ok s ctx priv e
-  (* | E_CTransError: ∀ l1 l2 l s ctx priv (e: env s) (f: trans_func l1 l2), *)
-
+Reserved Notation "c1 '>[' f ']>' c2" (at level 50, no associativity).
+Inductive step_cell: ∀ ℓ1 ℓ2, trans_func ℓ1 ℓ2 → config → config → Prop :=
+  (* If the environment is empty, then we cannot do anything.  *)
+  | E_CTransSkip1:
+      ∀ ℓ1 ℓ2 s Γ β e (f: trans_func ℓ1 ℓ2), 
+          List.length e = 0 →
+          ⟨ s Γ β e ⟩ >[ f ]> ⟨ s Γ β e ⟩
+  (* If the environment is not empty but there is no active tuples, we cannot do anything. *)
+  | E_CTransSkip2:
+      ∀ ℓ1 ℓ2 s Γ β e (f: trans_func ℓ1 ℓ2) (non_empty: List.length e > 0) tl,
+          tl = (env_slice_get_tuples (get_env_slice s e non_empty)) →
+          List.length tl = 0 → 
+          ⟨ s Γ β e ⟩ >[ f ]> ⟨ s Γ β e ⟩
+  (* No active labels are found; this should be an error. *)
+  | E_CTransError:
+      ∀ ℓ1 ℓ2 s Γ β e (f: trans_func ℓ1 ℓ2) (non_empty: List.length e > 0)
+        tl (tl_non_empty: List.length tl > 0) t c_idx,
+          (* tl => A list of tuples. *)
+          tl = (env_slice_get_tuples (get_env_slice s e non_empty)) →
+          (* t => The first tuple. *)
+          t = hd_ok tl tl_non_empty →
+          (* we now get the label encodings. *)
+          None = Policy.label_lookup c_idx Γ →
+          ⟨ s Γ β e ⟩ >[ f ]> config_error
+  (* The label does not flow to the current one. *)
+  | E_CTransInvalid:
+      ∀ ℓ1 ℓ2 ℓcur ℓdisc s Γ β e (f: trans_func ℓ1 ℓ2) (non_empty: List.length e > 0)
+        tl (tl_non_empty: List.length tl > 0) t c_idx,
+          (* tl => A list of tuples. *)
+          tl = (env_slice_get_tuples (get_env_slice s e non_empty)) →
+          (* t => The first tuple. *)
+          t = hd_ok tl tl_non_empty →
+          (* we now get the label encodings. *)
+          Some (ℓcur, Some ℓdisc) = Policy.label_lookup c_idx Γ →
+          ~ (ℓcur ⊑ ℓ1) →
+          ⟨ s Γ β e ⟩ >[ f ]> ⟨ s Γ β e ⟩
+  (* This transition is ok. *)
+  | E_CTransOk:
+      ∀ ℓ1 ℓ2 ℓcur ℓdisc s Γ β e (f: trans_func ℓ1 ℓ2) (non_empty: List.length e > 0)
+        tl (tl_non_empty: List.length tl > 0) t c_idx,
+          (* tl => A list of tuples. *)
+          tl = (env_slice_get_tuples (get_env_slice s e non_empty)) →
+          (* t => The first tuple. *)
+          t = hd_ok tl tl_non_empty →
+          (* we now get the label encodings. *)
+          Some (ℓcur, Some ℓdisc) = Policy.label_lookup c_idx Γ →
+          (* we now get the label encodings. *)
+          ℓcur ⊑ ℓ1 →
+          (* TODO: Update the policy encoding as well as the environment. *)
+          ⟨ s Γ β e ⟩ >[ f ]> ⟨ s Γ β e ⟩
 where "c1 '>[' f ']>' c2" := (step_cell _ _ f c1 c2).
-
-Notation "{{ ctx priv env }}":= (config_ok _ ctx priv env) (at level 50, left associativity) .
 
 (* 
   `step_config` is an inductive type representing the transition rules for configurations. 
@@ -105,17 +178,17 @@ Notation "{{ ctx priv env }}":= (config_ok _ ctx priv env) (at level 50, left as
   - `E_Error`   : If the configuration is error, it remains error.
   ...
 *)
-Reserved Notation "c1 '=[' o ']=>' c2" (at level 50).
+Reserved Notation "c1 '=[' o ']=>' c2" (at level 50, left associativity).
 Inductive step_config: Operator → config → config → Prop :=
   (* Empty operator clears the environment. *)
-  | E_Empty: ∀ s1 s2 ctx priv (e: env s1), config_ok s1 ctx priv e =[ operator_empty ]=> config_ok s2 ctx priv nil
+  | E_Empty: ∀ s1 s2 Γ β (e: ℰ s1),
+      ⟨ s1 Γ β e ⟩ =[ operator_empty ]=> ⟨ s2 Γ β nil ⟩
   (* If the operator returns an empty environment, we do nothing. *)
-  | E_ProjEmpty: ∀ s1 s2 ctx ctx' priv priv' (e: env s1) (e': env s2) project_list o,
-      config_ok s1 ctx priv e =[ o ]=> config_ok s2 ctx' priv' e' →
-      List.length e' = 0 →
-      config_ok s1 ctx priv e =[ operator_project project_list o ]=> config_ok s2 ctx' priv' nil
-  | E_Proj: ∀ s1 s2 ctx ctx' priv priv' (e: env s1) (e': env s2) project_list o,
-      config_ok s1 ctx priv e =[ o ]=> config_ok s2 ctx' priv' e' →
+  | E_ProjEmpty: ∀ s1 s2 Γ Γ' β β' (e: ℰ s1) (e': ℰ s2) project_list o,
+      ⟨ s1 Γ β e ⟩ =[ o ]=> ⟨ s2 Γ' β' e' ⟩ →
+      ⟨ s1 Γ β e ⟩ =[ operator_project project_list o ]=> ⟨ s2 Γ' β' nil ⟩
+  | E_Proj: ∀ s1 s2 Γ Γ' β β' (e: ℰ s1) (e': ℰ s2) project_list o,
+      ⟨ s1 Γ β e ⟩ =[ o ]=> ⟨ s2 Γ' β' e' ⟩ →
       List.length e' > 0 →
-      config_ok s1 ctx priv e =[ operator_project project_list o]=> config_ok s2 ctx' priv' e'
+      ⟨ s1 Γ β e ⟩ =[ operator_project project_list o]=> ⟨ s2 Γ' β' e' ⟩
 where "c1 '=[' o ']=>' c2" := (step_config o c1 c2).
