policy_proof/coq/security.v
@@ -5,7 +5,7 @@ Require Import query.
 Require Import types.
 
 (* todo *)
-Fixpoint env_ok s (e : env s) : Prop :=
+Fixpoint env_ok s (e : ℰ s) : Prop :=
   match e with
     | nil => True
     | (x, t) :: e' =>  False ∨ env_ok _ e'
@@ -13,10 +13,10 @@ Fixpoint env_ok s (e : env s) : Prop :=
 
 (* todo *)
 Theorem secure_query:
-  ∀ s s' ctx ctx' priv priv' e e' o c,
-    config_ok s ctx priv e =[ o ]=> c →
+  ∀ s s' Γ Γ' β β' e e' o c,
+    config_ok s Γ β e =[ o ]=> c →
       c = config_error ∨
-      c = config_ok s' ctx' priv' e' ∧ env_ok s' e'.
+      c = config_ok s' Γ' β' e' ∧ env_ok s' e'.
 Proof.
   intros.
 Admitted.
